src/fib/Theory.v
@@ -11,12 +11,50 @@ Definition fibonacci (fib : N -> N) :=
   fib 1 = 1
   /\
   forall n : N,
-    fib (N.succ (N.succ n)) = fib (N.succ n) + fib n.
+    fib (n + 2) = fib (n + 1) + fib n.
+
+(* Implementation of the fibonacci sequence *)
+
+(*
+Fixpoint fib (n:nat) : nat :=
+  match n with
+  | 0 ⇒ 0
+  | S n´ ⇒
+    match n´ with
+    | 0 ⇒ 1
+    | S n´´ ⇒ fib n´ + fib n´´
+    end
+  end.
+*)
+
+
+Fixpoint fib (n : N) : N :=
+  match n with
+  | 0 => 0
+  | Npos p as n' =>
+    match p with
+    | xH => 1
+    | _ => fib (N.pred n') + fib (N.pred (N.pred n'))
+    end
+  end.
+
+Theorem fib_impl : fibonacci fib.
+Proof.
+  unfold fibonacci.
+  simpl.
+  split.
+  reflexivity.
+  split. reflexivity.
+  intros.
+  induction n.
+  - simpl. reflexivity.
+  - simpl.
+Qed.
 
 (*
   Here we prove that the value of `curr` always matches (fib n)
 *)
 Theorem implements_fib : forall (base s : State),
-    reachable base s -> curr s == fib (n s).
+    reachable base s -> curr s = fib (n s).
 Proof
 Qed.
